quickchick again

coq-minuska/theories/playground.v
@@ -1,139 +1,17 @@
 From Minuska Require Import
     prelude
     spec
-    specb
-    default_static_model
-    builtin.int_signature
-    builtin.int_model
-    pi.trivial
-    symex
-.
-About stdpp.strings.String.
-Locate String.
-From QuickChick Require Import QuickChick.
-Import QcDefaultNotation.
-
-#[local]
-Instance Σ : StaticModel := @default_model int_signature (int_model _ _ _) MyProgramInfo.
-
-#[local]
-Instance show_builtin : Show builtin_value := {|
-    show := fun x => match x with inl b => show b | inr z => show z end
-|}.
-
-Definition genBuiltin : G builtin_value :=
-    oneOf_ (returnGen (inl true)) [(returnGen (inl true)); (returnGen (inl false)); (returnGen (inr 1%Z));(returnGen (inr 2%Z))]
+    basic_properties
+    quickchick_setup
+    (* symex *)
+    substitution_parallel
 .
 
-#[local]
-Instance show_symbol : Show symbol := {|
-    show := fun x => x;
-|}.
-
-Fixpoint show_to {T : Type} {_ST : Show T} (t : TermOver T) : string  :=
-    match t with
-    | t_over b => show b
-    | t_term s l => show s +:+ "[" +:+ (concat "," (show_to <$> l ))  +:+ "]"
-    end
-.
-
-#[local]
-Instance showTerm {T : Type} {_ST : Show T} : Show (TermOver T) := {|
-    show := show_to ;
-|}.
-
-Definition genVariable : G variable :=
-    oneOf [ret "x"; ret "y"; ret "z"; ret "xx"; ret "yy"; ret "zz"]
-.
-
-Definition genSymbol : G symbol :=
-    (oneOf [(returnGen "s");(returnGen "t");(returnGen "a");(returnGen "b");(returnGen "c")])
-.
-
-(* Print IntFunSymbol. *)
-(* Compute builtin_function_symbol. *)
-
-Definition genFunction : G builtin_function_symbol :=
-    elems [int_plus; int_minus; int_uminus; int_zero; int_one; int_eq; int_le; int_lt]
-.
-
-Fixpoint genTermSized' {T : Type} (sz : nat) (g : nat -> G T) : G (TermOver T) :=
-  match sz with
-    | O => bindGen (g sz) (fun x => returnGen (t_over x))
-    | S sz' =>
-        freq [ (1, bindGen (g sz) (fun x => returnGen (t_over x))) ;
-                (sz, bindGen genSymbol
-                (fun s => bindGen (listOf (genTermSized' sz' g)) (fun l => returnGen (t_term s l))))
-             ]
-  end.
-
-Definition genTermSized sz := genTermSized' sz (fun _ => genBuiltin).
-(* Sample (genTermSized 3). *)
-(* Print Expression2. *)
-
-#[local]
-Instance showFun : Show builtin_function_symbol := {|
-    show := fun f => match (f : builtin_function_symbol) with
-    | int_plus => "plus"
-    | int_minus => "minus"
-    | int_uminus => "uminus"
-    | int_zero => "zero"
-    | int_one => "one"
-    | int_eq => "eq"
-    | int_le => "le"
-    | int_lt => "lt"
-    end ;
-|}.
-
-#[local]
-Instance showQery : Show QuerySymbol := {|
-    show := fun q => match (q : QuerySymbol) with
-    | qs_program => "qs_program"
-    end ;
-|}.
-
-
-Fixpoint show_e (e : Expression2) : string  :=
-    match e with
-    | e_ground g => show g
-    | e_variable x => show x
-    | e_fun f l => show f +:+ "(" +:+ (concat "," (show_e <$> l ))  +:+ ")"
-    | e_query q l => show q +:+ "(" +:+ (concat "," (show_e <$> l ))  +:+ ")"
-    end
-.
-
-#[local]
-Instance showExpr : Show (Expression2) := {|
-    show := show_e ;
-|}.
-
-
-Fixpoint genExprSized (sz : nat) : G (Expression2) :=
-  match sz with
-    | O => oneOf [(bindGen genVariable (fun x => returnGen (e_variable x))); bindGen (genTermSized sz) (fun x => returnGen (e_ground x))]
-    | S sz' =>
-        freq [
-            (1,
-                oneOf [(bindGen genVariable (fun x => returnGen (e_variable x))); bindGen (genTermSized sz) (fun x => returnGen (e_ground x))]
-            );
-            (sz, 
-                bindGen (listOf (genExprSized sz')) (fun l =>
-                    bindGen (genFunction) (fun f =>
-                        ret (e_fun f l)
-                    )
-                )
-            )
-        ]
-  end.
-
-
-Definition genTermOverExprSized sz := genTermSized' sz genExprSized.
-
-Definition genValuationSized (sz : nat) : G (gmap variable (TermOver builtin_value)) :=
+Definition genSubstitutionSized (sz : nat) : G (gmap variable (TermOver BuiltinOrVar)) :=
     bindGen (
         listOf (
             bindGen genVariable (fun x =>
-                bindGen (genTermSized sz) (fun g =>
+                bindGen (genPatternSized sz) (fun g =>
                     returnGen (x, g)
                 )
             )
@@ -141,17 +19,23 @@ Definition genValuationSized (sz : nat) : G (gmap variable (TermOver builtin_val
     ) (fun l => returnGen (list_to_map l))
 .
 
-
-Definition showVal_ (ρ : Valuation2) : string :=
-        let l := map_to_list ρ in
-        show (l)
-.
-(* About map_to_list. *)
 #[local]
-Instance showVal : Show Valuation2 := {|
-    show := showVal_
-|}.
+Instance subp_eqdec : EqDecision SubP.
+Proof.
+    apply _.
+Defined.
 
+Sample (genSubstitutionSized 3).
+
+QuickChick (forAll (genSubstitutionSized 3)(fun a =>
+    forAll (genSubstitutionSized 3)(fun b =>
+        forAll (genSubstitutionSized 3)(fun c =>
+            bool_decide (subp_compose (subp_compose a b) c = subp_compose a (subp_compose b c))
+        )
+    )
+)).
+
+(* 
 (* Sample (genValuationSized 1). *)
 (* Search bool. *)
 Definition replace_and_collect_property_1
@@ -225,4 +109,4 @@ Definition myP2 := forAll
 QuickChick (
     myP2
 ).
-(* replace_and_collect *)
+replace_and_collect *)
